policy_proof/coq/security.v
@@ -118,4 +118,5 @@ Proof.
               --- simpl. intros. discriminate.
               --- simpl. reflexivity.
               --- simpl. econstructor.
+
 Admitted.
